Tactics/PruneUpdates.lean
@@ -1,0 +1,449 @@
+/-
+Copyright (c) 2024 Amazon.com, Inc. or its affiliates. All Rights Reserved.
+Released under Apache 2.0 license as described in the file LICENSE.
+Author(s): Shilpi Goel
+-/
+
+import Tactics.PruneUpdatesLogic
+import Tactics.Attr
+
+import Lean
+
+namespace ArmConstr
+
+open Lean Elab Tactic Expr Meta
+
+abbrev ArmExpr := ArmConstr.Expr
+abbrev ArmStateVar := ArmConstr.StateVar
+abbrev ArmUpdate := ArmConstr.Update
+abbrev ArmUpdates := ArmConstr.Updates
+
+section Tracing
+-- (FIXME): Move to Sym/Common.lean?
+
+variable {α : Type} {m : Type → Type} [Monad m] [MonadTrace m] [MonadLiftT IO m]
+  [MonadRef m] [AddMessageContext m] [MonadOptions m] {ε : Type}
+  [MonadAlwaysExcept ε m] [MonadLiftT BaseIO m]
+
+/-- Add a trace node with the `Tactic.prune_updates` trace class -/
+def withTraceNode (msg : MessageData) (k : m α)
+    (collapsed : Bool := true)
+    (tag : String := "")
+    : m α := do
+  Lean.withTraceNode `Tactic.prune_updates (fun _ => pure msg) k collapsed tag
+
+end Tracing
+
+/-! ## Mapping Arm State Update Expressions to Lean Expressions -/
+
+def ArmStateVar.toExpr (s : ArmStateVar) : Lean.Expr :=
+  mkNatLit s
+
+instance : ToExpr ArmStateVar where
+  toExpr a := a.toExpr
+  toTypeExpr := mkConst ``ArmConstr.StateVar
+
+def ArmUpdate.toExpr (u : ArmUpdate) : Lean.Expr :=
+  open ArmConstr.Update in
+  match u with
+  | .err v => mkAppN (mkConst ``err) #[(mkNatLit v)]
+  | .pc v => mkAppN (mkConst ``pc) #[(mkNatLit v)]
+  | .gpr i v => mkAppN (mkConst ``gpr)
+                       #[(Lean.toExpr i), (mkNatLit v)]
+  | .sfp i v => mkAppN (mkConst ``sfp)
+                        #[(Lean.toExpr i), (mkNatLit v)]
+  | .flag i v => mkAppN (mkConst ``flag)
+                        #[(Lean.toExpr i), (mkNatLit v)]
+
+instance : ToExpr ArmUpdate where
+  toExpr a := a.toExpr
+  toTypeExpr := mkConst ``ArmConstr.Update
+
+def ArmUpdates.toExpr (us : ArmUpdates) : Lean.Expr :=
+  match us with
+  | [] => Lean.toExpr ([] : Updates)
+  | u :: rest =>
+    mkAppN (mkConst ``List.cons [levelZero])
+          #[mkConst ``Update, (Lean.toExpr u), (ArmUpdates.toExpr rest)]
+
+instance : ToExpr ArmUpdates where
+  toExpr a := a.toExpr
+  toTypeExpr := mkConst ``ArmConstr.Updates
+
+def ArmExpr.toExpr (e : ArmExpr) : Lean.Expr :=
+  mkApp3 (mkConst ``ArmConstr.Expr.mk)
+         (ArmStateVar.toExpr e.curr_state)
+         (ArmStateVar.toExpr e.prev_state)
+         (ArmUpdates.toExpr e.writes)
+
+instance : ToExpr ArmExpr where
+  toExpr a := a.toExpr
+  toTypeExpr := mkConst ``ArmConstr.Expr
+
+/-
+def foo : Lean.Expr :=
+  open ArmExpr in
+  ArmExpr.toExpr { curr_state := 1, prev_state := 0, writes := [.gpr 1#5 (0), .err (0)] }
+
+#eval foo
+
+elab "foo" : term => return foo
+
+#eval foo
+-/
+
+/-! ## Mapping Lean Expressions to Arm State Update Expressions -/
+
+namespace ToArmExpr
+
+/- Borrowed from: Lean/Meta/Tactic/LinearArith/Nat/Basic.lean -/
+structure State where
+   -- It should be fine to use `KExprMap` here because the mapping should be
+   -- small and few HeadIndex collisions.
+  stateVarMap  : KExprMap ArmStateVar := {}
+  stateVars    : Array Lean.Expr := #[]
+  gprVarMap    : KExprMap GPRVar := {}
+  gprVars      : Array Lean.Expr := #[]
+  sfpVarMap    : KExprMap SFPVar := {}
+  sfpVars      : Array Lean.Expr := #[]
+  flagVarMap   : KExprMap FlagVar := {}
+  flagVars     : Array Lean.Expr := #[]
+  errVarMap    : KExprMap ErrVar := {}
+  errVars      : Array Lean.Expr := #[]
+  pcVarMap     : KExprMap PCVar := {}
+  pcVars       : Array Lean.Expr := #[]
+
+abbrev M := StateRefT State MetaM
+
+def addAsStateVar (e : Lean.Expr) : M ArmStateVar := do
+  if let some x ← (← get).stateVarMap.find? e then
+    return x
+  else
+    let x := (← get).stateVars.size
+    let s ← get
+    set { s with stateVarMap := (← s.stateVarMap.insert e x),
+                 stateVars := s.stateVars.push e : State }
+    return x
+
+def addAsPCVar (e : Lean.Expr) : M Nat := do
+  if let some x ← (← get).pcVarMap.find? e then
+    return x
+  else
+    let x := (← get).pcVars.size
+    let s ← get
+    set { s with pcVarMap := (← s.pcVarMap.insert e x),
+                 pcVars := s.pcVars.push e : State }
+    return x
+
+def addAsErrVar (e : Lean.Expr) : M Nat := do
+  if let some x ← (← get).errVarMap.find? e then
+    return x
+  else
+    let x := (← get).errVars.size
+    let s ← get
+    set { s with errVarMap := (← s.errVarMap.insert e x),
+                 errVars := s.errVars.push e : State }
+    return x
+
+def addAsGPRVar (e : Lean.Expr) : M Nat := do
+  if let some x ← (← get).gprVarMap.find? e then
+    return x
+  else
+    let x := (← get).gprVars.size
+    let s ← get
+    set { s with gprVarMap := (← s.gprVarMap.insert e x),
+                 gprVars := s.gprVars.push e : State }
+    return x
+
+def addAsSFPVar (e : Lean.Expr) : M Nat := do
+  if let some x ← (← get).sfpVarMap.find? e then
+    return x
+  else
+    let x := (← get).sfpVars.size
+    let s ← get
+    set { s with sfpVarMap := (← s.sfpVarMap.insert e x),
+                 sfpVars := s.sfpVars.push e : State }
+    return x
+
+def addAsFlagVar (e : Lean.Expr) : M Nat := do
+  if let some x ← (← get).flagVarMap.find? e then
+    return x
+  else
+    let x := (← get).flagVars.size
+    let s ← get
+    set { s with flagVarMap := (← s.flagVarMap.insert e x),
+                 flagVars := s.flagVars.push e : State }
+    return x
+
+instance : ToMessageData ArmExpr where
+  toMessageData x := m!"\{curr: {x.curr_state}; writes: {x.writes} prev: {x.prev_state}}"
+
+def getPFlagValue? (e : Lean.Expr) : MetaM (Option PFlag) := OptionT.run do
+  match_expr e with
+  | PFlag.N => return PFlag.N
+  | PFlag.Z => return PFlag.Z
+  | PFlag.C => return PFlag.C
+  | PFlag.V => return PFlag.V
+  | _ => failure
+
+partial def toArmUpdatesAndStateVar (curr_state writes : Lean.Expr) (us : ArmUpdates) :
+  M (ArmStateVar × ArmUpdates × ArmStateVar) :=
+  withTraceNode m!"toArmUpdatesAndStateVar" (tag := "toArmUpdatesAndStateVar") <| do
+  match_expr writes with
+  | w fld val rest =>
+    let (update : ArmUpdate) ←
+      match_expr fld with
+      | StateField.ERR =>
+        let var ← addAsErrVar val
+        trace[Tactic.prune_updates] "Adding ERR value {val} as {var}"
+        trace[Tactic.prune_updates] "All variables in the Err map: {(← get).errVars}"
+        pure (Update.err var)
+      | StateField.PC =>
+        let var ← addAsPCVar val
+        trace[Tactic.prune_updates] "Adding PC value {val} as {var}"
+        trace[Tactic.prune_updates] "All variables in the PC map: {(← get).pcVars}"
+        pure (Update.pc var)
+      | StateField.GPR i =>
+        let some ⟨n, i'⟩ ← getBitVecValue? i | failure
+        let var ← addAsGPRVar val
+        trace[Tactic.prune_updates] "Adding GPR value {val} as {var}"
+        trace[Tactic.prune_updates] "All variables in the GPR map: {(← get).gprVars}"
+        if h : n = 5 then
+            pure (Update.gpr (i'.cast h) var)
+        else failure
+      | StateField.SFP i =>
+        let some ⟨n, i'⟩ ← getBitVecValue? i | failure
+        let var ← addAsSFPVar val
+        trace[Tactic.prune_updates] "Adding SFP value {val} as {var}"
+        trace[Tactic.prune_updates] "All variables in the SFP map: {(← get).sfpVars}"
+        if h : n = 5 then
+            pure (Update.sfp (i'.cast h) var)
+        else failure
+      | StateField.FLAG i =>
+        let some i' ← getPFlagValue? i | failure
+        let var ← addAsFlagVar val
+        trace[Tactic.prune_updates] "Adding FLAG value {val} as {var}"
+        trace[Tactic.prune_updates] "All variables in the Flag map: {(← get).flagVars}"
+        pure (Update.flag i' var)
+      | _ => failure
+    toArmUpdatesAndStateVar curr_state rest (us ++ [update])
+  | _ =>
+    -- writes is just a state var at this point.
+    let (prev_state_var : ArmStateVar) ← addAsStateVar writes
+    let (curr_state_var : ArmStateVar) ← addAsStateVar curr_state
+    trace[Tactic.prune_updates] "Current State: {curr_state} var: {curr_state_var}"
+    trace[Tactic.prune_updates] "Previous State: {writes} var: {prev_state_var}"
+    trace[Tactic.prune_updates] "All Updates: {us}"
+    return (curr_state_var, us, prev_state_var)
+
+partial def toArmExpr? (e : Lean.Expr) : M (Option ArmExpr) :=
+  withTraceNode m!"toArmExpr?" (tag := "toArmExpr?") <| do
+  match_expr e with
+  | Eq α s writes =>
+    let_expr ArmState ← α | failure
+    let (curr_state, writes, prev_state) ← toArmUpdatesAndStateVar s writes []
+    return some { curr_state, writes, prev_state }
+  | _ => failure
+
+def run (x : M α) : MetaM (α × State) := do
+  let (a, s) ← x.run {}
+  return (a, s)
+
+end ToArmExpr
+
+def toContextExpr (s : ToArmExpr.State) : MetaM Lean.Expr :=
+  withTraceNode m!"toContextExpr" (tag := "toContextExpr") <| do
+  let state_ctx ← mkListLit (mkConst ``ArmState) s.stateVars.toList
+  let err_ctx   ← (mkListLit (mkConst ``StateError) s.errVars.toList)
+  let pc_ctx    ← (mkListLit (← mkAppM ``BitVec #[mkNatLit 64]) s.pcVars.toList)
+  let gpr_ctx   ← (mkListLit (← mkAppM ``BitVec #[mkNatLit 64]) s.gprVars.toList)
+  let sfp_ctx   ← (mkListLit (← mkAppM ``BitVec #[mkNatLit 128]) s.sfpVars.toList)
+  let flag_ctx  ← (mkListLit (← mkAppM ``BitVec #[mkNatLit 1]) s.flagVars.toList)
+  let ans := (mkAppN (mkConst ``ArmConstr.Context.mk)
+                      #[state_ctx, err_ctx, pc_ctx, gpr_ctx, sfp_ctx, flag_ctx])
+  trace[Tactic.prune_updates] m!"ArmConstr.Context: {ans}"
+  return ans
+
+abbrev mkAuxDecl := Lean.Elab.Tactic.BVDecide.Frontend.mkAuxDecl
+
+-- (FIXME) Better formatting; change into code action, etc.!
+def toArmMessageData (e : Expr) (s : ToArmExpr.State) : MessageData :=
+  let curr_state := s.stateVars[e.curr_state]!
+  let prev_state := s.stateVars[e.prev_state]!
+  let writes := go e.writes prev_state s 0
+  m!"{curr_state} = {writes}"
+  where go (us : Updates) (prev_state : Lean.Expr)
+           (s : ToArmExpr.State) (paren_count : Nat) :=
+    match us with
+    | [] =>
+        let closing_parens := List.asString (List.replicate paren_count ')')
+        m!"{prev_state}{closing_parens}"
+    | u :: rest =>
+      let m :=
+        match u with
+        | .err v => m!"(w .ERR ({s.errVars[v]!}) "
+        | .pc v => m!"(w .PC ({s.pcVars[v]!}) "
+        | .gpr i v => m!"(w (.GPR {i}) ({s.gprVars[v]!}) "
+        | .sfp i v => m!"(w (.SFP {i}) ({s.sfpVars[v]!}) "
+        | .flag i v => m!"(w (.FLAG {i}) ({s.flagVars[v]!}) "
+      m!"{m} {go rest prev_state s (1 + paren_count)}"
+
+def ArmExprPruned? (refl_proof_name : Name) (e : Lean.Expr) :
+  MetaM (Option (Lean.Expr × Lean.Expr)) :=
+  withTraceNode m!"ArmExprPruned?" (tag := "ArmExprPruned?") <| do
+  let validate ←(getBoolOption `Tactic.prune_updates.validate)
+  let (some arm_expr, state) ←
+    ToArmExpr.run (ToArmExpr.toArmExpr? e) | return none
+  trace[Tactic.prune_updates] "Arm Expr: {arm_expr}"
+  trace[Tactic.prune_updates] "State Context: {state.stateVars}"
+  trace[Tactic.prune_updates] "ERR Context: {state.errVars}"
+  trace[Tactic.prune_updates] "PC Context: {state.pcVars}"
+  trace[Tactic.prune_updates] "GPR Context: {state.gprVars}"
+  trace[Tactic.prune_updates] "SFP Context: {state.sfpVars}"
+  trace[Tactic.prune_updates] "Flag Context: {state.flagVars}"
+  let arm_expr_pruned := arm_expr.prune
+  trace[Tactic.prune_updates] "Pruned Arm Expr: {arm_expr_pruned}"
+
+  let ctx_expr ← toContextExpr state
+  if validate then
+    check ctx_expr
+    trace[Tactic.prune_updates] "Checked context expressions: {ctx_expr}"
+
+  let answer := toArmMessageData arm_expr_pruned state
+  trace[Tactic.prune_updates.answer] "Pruned Answer: {answer}"
+
+  let auxValue := mkApp2 (mkConst ``ArmConstr.Expr.isPruned)
+                         (toExpr arm_expr) (toExpr arm_expr_pruned)
+  trace[Tactic.prune_updates] "Aux Value: {auxValue}"
+  mkAuxDecl refl_proof_name auxValue (mkConst ``Bool)
+
+  let refl_proof :=
+    mkApp3
+    (mkConst ``Lean.ofReduceBool)
+    (mkConst refl_proof_name)
+    (toExpr true)
+    (← mkEqRefl (toExpr true))
+
+  if validate then
+    check refl_proof
+    trace[Tactic.prune_updates] "Checked reflection proof: {refl_proof}"
+
+  let p := mkAppN (mkConst ``ArmConstr.Expr.eq_true_of_denote)
+                    #[ctx_expr,
+                      (toExpr arm_expr),
+                      (toExpr arm_expr_pruned),
+                      refl_proof]
+  if validate then
+    check p
+    trace[Tactic.prune_updates] "Checked proof: {p}"
+  return some (mkConst ``True, p)
+
+def ReflectionProofName : Lean.Elab.TermElabM Name := do
+  Lean.Elab.Term.mkAuxName `_armexpr_reflection_def
+
+open Lean.Elab.Tactic in
+elab "prune_updates" h_state_eq:term : tactic =>
+  withTraceNode m!"prune_updates" (tag := "prune_updates") <| withMainContext do
+  trace[Tactic.prune_updates] "h_state_eq: {h_state_eq}"
+  let h_state_eq_expr ← elabTerm h_state_eq none
+  let hStateEq ← inferType h_state_eq_expr
+  trace[Tactic.prune_updates] "hStateEq: {hStateEq}"
+  let refl_proof_name ← ReflectionProofName
+  let some (_, e) ← ArmExprPruned? refl_proof_name hStateEq | return
+  trace[Tactic.prune_updates] "Ctor of Proof after ArmExprPruned?: {e.ctorName}"
+  trace[Tactic.prune_updates] "Proof after ArmExprPruned?: {e}"
+  /-
+  The rest of this code is heavily borrowed from `myApply` in Metaprogramming in
+  Lean 4
+  (https://leanprover-community.github.io/lean4-metaprogramming-book/main/04_metam.html)
+  -/
+  let goal ← Lean.Elab.Tactic.getMainGoal
+  let target ← goal.getType
+  let type ← inferType e
+  trace[Tactic.prune_updates] "Target: {target}"
+  trace[Tactic.prune_updates] "Proof, after `inferType`: {type}"
+  -- If `type` has the form `∀ (x₁ : T₁) ... (xₙ : Tₙ), U`, introduce new
+  -- metavariables for the `xᵢ` and obtain the conclusion `U`. (If `proof_type` does
+  -- not have this form, `args` is empty and `conclusion = type`.)
+  let (args, _, conclusion) ← forallMetaTelescopeReducing type
+  trace[Tactic.prune_updates] "Args: {args}"
+  trace[Tactic.prune_updates] "Conclusion: {conclusion}"
+  if ← isDefEq target conclusion then
+    trace[Tactic.prune_updates] "Target and conclusion are DefEq!"
+    -- Assign the goal to `e x₁ ... xₙ`, where the `xᵢ` are the fresh
+    -- metavariables in `args`.
+    if ← isDefEq args[0]! h_state_eq_expr then
+    trace[Tactic.prune_updates] "Args[0]! and h_state_eq_expr are DefEq!"
+    let new_goal_term := mkAppN e args
+    trace[Tactic.prune_updates] "New Goal: {new_goal_term}"
+    goal.assign new_goal_term
+    -- `isDefEq` may have assigned some of the `args`. Report the rest as new
+    -- goals.
+    let newGoals ← args.filterMapM λ mvar => do
+      let mvarId := mvar.mvarId!
+      if ! (← mvarId.isAssigned) && ! (← mvarId.isDelayedAssigned) then
+        return some mvarId
+      else
+        return none
+    trace[Tactic.prune_updates] "newGoals: {newGoals.toList}"
+    setGoals newGoals.toList
+  else
+    -- If the conclusion does not unify with the target, throw an error.
+    throwTacticEx `prune_updates goal m!"{e} is not applicable to goal with target {target}"
+
+namespace ArmConstr
+
+section Tests
+
+#time
+-- set_option trace.Tactic.prune_updates.answer true in
+private theorem example1
+  (h_s1 : s1 = w (.GPR 0#5) x0 (w (.GPR 1#5) x1 (w (.GPR 0#5) x1 s0))) :
+  s1 = (w (.GPR 0x00#5) x0  (w (.GPR 0x01#5) x1  s0)) := by
+  prune_updates h_s1
+  done
+
+-- #print example1
+
+#time
+private theorem example2
+  (h_s1 : s1 = w (.GPR 1#5) (x100 + x100') (w (.GPR 0#5) x500 (w (.GPR 8#5) x1 s0))) :
+  s1 = w (.GPR 0#5) x500 (w (.GPR 1#5) (x100 + x100') (w (.GPR 8#5) x1 s0)) := by
+  prune_updates h_s1
+  done
+
+#time
+-- set_option trace.Tactic.prune_updates.answer true in
+private theorem example3
+  (h_s1 : s1 =
+   (w StateField.PC (if ¬r (StateField.GPR 0x2#5) s = 0x0#64 then 0x126500#64 else 0x126c94#64)
+    (w (StateField.SFP 0x3#5)
+      (DPSFP.binary_vector_op_aux 0 2 64 BitVec.add (r (StateField.SFP 0x3#5) s) (r (StateField.SFP 0x1d#5) s) 0x0#128)
+      (w StateField.PC 0x126c8c#64
+        (w (StateField.SFP 0x2#5)
+          (DPSFP.binary_vector_op_aux 0 2 64 BitVec.add (r (StateField.SFP 0x2#5) s) (r (StateField.SFP 0x1c#5) s)
+            0x0#128)
+          (w StateField.PC 0x126c88#64
+            (w (StateField.SFP 0x1#5)
+              (DPSFP.binary_vector_op_aux 0 2 64 BitVec.add (r (StateField.SFP 0x1#5) s) (r (StateField.SFP 0x1b#5) s)
+                0x0#128)
+              (w StateField.PC 0x126c84#64
+                (w (StateField.SFP 0x0#5)
+                  (DPSFP.binary_vector_op_aux 0 2 64 BitVec.add (r (StateField.SFP 0x0#5) s)
+                    (r (StateField.SFP 0x1a#5) s) 0x0#128)
+                  s))))))))) :
+  s1 = (w .PC (if ¬r (StateField.GPR 2#5) s = 0#64 then 1205504#64
+    else
+      1207444#64)  (w (.SFP 0x00#5) (DPSFP.binary_vector_op_aux 0 2 64 BitVec.add (r (StateField.SFP 0#5) s)
+      (r (StateField.SFP 26#5) s)
+      0#128)  (w (.SFP 0x01#5) (DPSFP.binary_vector_op_aux 0 2 64 BitVec.add (r (StateField.SFP 1#5) s)
+      (r (StateField.SFP 27#5) s)
+      0#128)  (w (.SFP 0x02#5) (DPSFP.binary_vector_op_aux 0 2 64 BitVec.add (r (StateField.SFP 2#5) s)
+      (r (StateField.SFP 28#5) s)
+      0#128)  (w (.SFP 0x03#5) (DPSFP.binary_vector_op_aux 0 2 64 BitVec.add (r (StateField.SFP 3#5) s)
+      (r (StateField.SFP 29#5) s) 0#128)  s)))))
+  := by
+  prune_updates h_s1
+  done
+
+end Tests
